Support for CPUID_AVX + interop wrappers

vale/code/arch/x64/interop/Cpuid_stdcalls.fst
@@ -12,6 +12,10 @@ let check_adx_bmi2 () =
   let x, _ = Vale.Stdcalls.Cpuid.check_adx_bmi2 () in //This is a call to the interop wrapper
   x
 
+let check_avx () =  
+  let x, _ = Vale.Stdcalls.Cpuid.check_avx () in //This is a call to the interop wrapper
+  x
+
 let check_avx2 () =  
   let x, _ = Vale.Stdcalls.Cpuid.check_avx2 () in //This is a call to the interop wrapper
   x
