vale/code/arch/x64/interop/Vale.Stdcalls.Cpuid.fsti
@@ -192,7 +192,7 @@ let avx_pre : VSig.vale_pre 8 dom =
   fun (c:V.va_code)
     (va_s0:V.va_state)
     (sb:IX64.stack_buffer 8) ->
-      VC.va_req_check_avx2_stdcall c va_s0 IA.win (as_vale_buffer sb)
+      VC.va_req_check_avx_stdcall c va_s0 IA.win (as_vale_buffer sb)
 
 [@__reduce__] noextract
 let avx_post : VSig.vale_post 8 dom =
@@ -201,7 +201,7 @@ let avx_post : VSig.vale_post 8 dom =
     (sb:IX64.stack_buffer 8)
     (va_s1:V.va_state)
     (f:V.va_fuel) ->
-      VC.va_ens_check_avx2_stdcall c va_s0 IA.win (as_vale_buffer sb) va_s1 f
+      VC.va_ens_check_avx_stdcall c va_s0 IA.win (as_vale_buffer sb) va_s1 f
 
 (* The vale lemma doesn't quite suffice to prove the modifies clause
    expected of the interop layer *)
@@ -218,13 +218,13 @@ let avx_lemma'
        V.eval_code code va_s0 f va_s1 /\
        VSig.vale_calling_conventions_stdcall va_s0 va_s1 /\
        avx_post code va_s0 sb va_s1 f))
- = VC.va_lemma_check_avx2_stdcall code va_s0 IA.win (as_vale_buffer sb)
+ = VC.va_lemma_check_avx_stdcall code va_s0 IA.win (as_vale_buffer sb)
 
 (* Prove that vm_lemma' has the required type *)
 noextract
 let avx_lemma = as_t #(VSig.vale_sig_stdcall avx_pre avx_post) avx_lemma'
 noextract
-let code_avx = VC.va_code_check_avx2_stdcall IA.win
+let code_avx = VC.va_code_check_avx_stdcall IA.win
 
 (* Here's the type expected for the check_avx wrapper *)
 [@__reduce__] noextract
@@ -239,6 +239,59 @@ let lowstar_avx_t =
     _
     (W.mk_prediction code_avx dom [] (avx_lemma code_avx IA.win))
 
+(* Need to rearrange the order of arguments *)
+[@__reduce__] noextract
+let avx2_pre : VSig.vale_pre 8 dom =
+  fun (c:V.va_code)
+    (va_s0:V.va_state)
+    (sb:IX64.stack_buffer 8) ->
+      VC.va_req_check_avx2_stdcall c va_s0 IA.win (as_vale_buffer sb)
+
+[@__reduce__] noextract
+let avx2_post : VSig.vale_post 8 dom =
+  fun (c:V.va_code)
+    (va_s0:V.va_state)
+    (sb:IX64.stack_buffer 8)
+    (va_s1:V.va_state)
+    (f:V.va_fuel) ->
+      VC.va_ens_check_avx2_stdcall c va_s0 IA.win (as_vale_buffer sb) va_s1 f
+
+(* The vale lemma doesn't quite suffice to prove the modifies clause
+   expected of the interop layer *)
+[@__reduce__] unfold noextract
+let avx2_lemma'
+    (code:V.va_code)
+    (_win:bool)
+    (va_s0:V.va_state)
+    (sb:IX64.stack_buffer 8)
+ : Ghost (V.va_state & V.va_fuel)
+     (requires
+       avx2_pre code va_s0 sb)
+     (ensures (fun (va_s1, f) ->
+       V.eval_code code va_s0 f va_s1 /\
+       VSig.vale_calling_conventions_stdcall va_s0 va_s1 /\
+       avx2_post code va_s0 sb va_s1 f))
+ = VC.va_lemma_check_avx2_stdcall code va_s0 IA.win (as_vale_buffer sb)
+
+(* Prove that vm_lemma' has the required type *)
+noextract
+let avx2_lemma = as_t #(VSig.vale_sig_stdcall avx2_pre avx2_post) avx2_lemma'
+noextract
+let code_avx2 = VC.va_code_check_avx2_stdcall IA.win
+
+(* Here's the type expected for the check_avx wrapper *)
+[@__reduce__] noextract
+let lowstar_avx2_t =
+  IX64.as_lowstar_sig_t_weak_stdcall
+    Interop.down_mem
+    code_avx2
+    8
+    dom
+    []
+    _
+    _
+    (W.mk_prediction code_avx2 dom [] (avx2_lemma code_avx2 IA.win))
+
 [@ (CCConv "stdcall") ]
 val check_aesni : normal lowstar_aesni_t
 
@@ -249,4 +302,7 @@ val check_sha : normal lowstar_sha_t
 val check_adx_bmi2 : normal lowstar_adx_t
 
 [@ (CCConv "stdcall") ]
-val check_avx2 : normal lowstar_avx_t
+val check_avx : normal lowstar_avx_t
+
+[@ (CCConv "stdcall") ]
+val check_avx2 : normal lowstar_avx2_t
